cfi/classes.v
@@ -1,0 +1,47 @@
+Require Import ssreflect ssrfun ssrbool eqtype ssrnat.
+Require Import common.common.
+
+Section WithClasses.
+
+Context {t : machine_types}.
+
+Class cfi_id := {
+  id         : eqType;
+
+  word_to_id : word t -> option id;
+  id_to_word : id -> word t;
+  
+  id_to_wordK : forall x, word_to_id (id_to_word x) = Some x;
+  word_to_idK : forall w x, word_to_id w = Some x -> id_to_word x = w
+                             
+}.
+
+End WithClasses.
+
+Section ControlFlow.
+
+Context {t : machine_types}
+        {ids : @cfi_id t}.
+
+Variable cfg : id -> id -> bool.
+
+Definition valid_jmp w1 w2 :=
+  match word_to_id w1, word_to_id w2 with
+    | Some id1, Some id2 => cfg id1 id2
+    | _, _ => false
+  end.
+
+Lemma valid_jmp_true w1 w2 :
+  valid_jmp w1 w2 = true ->
+  exists id1 id2, 
+    word_to_id w1 = Some id1 /\
+    word_to_id w2 = Some id2.
+Proof.
+  unfold valid_jmp.
+  intro VALID.
+  destruct (word_to_id w1) eqn:W1, (word_to_id w2) eqn:W2;
+  try discriminate.
+  by eexists; eauto.
+Qed.
+
+End ControlFlow.
